refactor rotation even more

Clean/Gadgets/ByteDecomposition.lean
@@ -206,3 +206,103 @@ def circuit (offset : Fin 8) : FormalCircuit (F p) field Outputs := {
   completeness := completeness offset
 }
 end Gadgets.ByteDecomposition
+
+namespace Gadgets.U64ByteDecomposition
+variable {p : ℕ} [Fact p.Prime]
+variable [p_large_enough: Fact (p > 2^16 + 2^8)]
+
+instance : Fact (p > 512) := by
+  constructor
+  linarith [p_large_enough.elim]
+
+structure Outputs (F : Type) where
+  low : U64 F
+  high : U64 F
+
+instance : ProvableStruct Outputs where
+  components := [U64, U64]
+  to_components := fun { low, high } => .cons low (.cons high .nil)
+  from_components := fun (.cons low (.cons high .nil)) => { low, high }
+
+/--
+  Decompose every limb of a u64 into a low and a high part.
+  The low part is the least significant `offset` bits, and the high part is the most significant `8 - offset` bits.
+-/
+def u64_byte_decomposition (offset : Fin 8) (x : Var U64 (F p)) : Circuit (F p) (Var Outputs (F p)) := do
+  let ⟨x0, x1, x2, x3, x4, x5, x6, x7⟩ := x
+
+  let ⟨x0_l, x0_h⟩ ← subcircuit (Gadgets.ByteDecomposition.circuit offset) x0
+  let ⟨x1_l, x1_h⟩ ← subcircuit (Gadgets.ByteDecomposition.circuit offset) x1
+  let ⟨x2_l, x2_h⟩ ← subcircuit (Gadgets.ByteDecomposition.circuit offset) x2
+  let ⟨x3_l, x3_h⟩ ← subcircuit (Gadgets.ByteDecomposition.circuit offset) x3
+  let ⟨x4_l, x4_h⟩ ← subcircuit (Gadgets.ByteDecomposition.circuit offset) x4
+  let ⟨x5_l, x5_h⟩ ← subcircuit (Gadgets.ByteDecomposition.circuit offset) x5
+  let ⟨x6_l, x6_h⟩ ← subcircuit (Gadgets.ByteDecomposition.circuit offset) x6
+  let ⟨x7_l, x7_h⟩ ← subcircuit (Gadgets.ByteDecomposition.circuit offset) x7
+
+  let low := U64.mk x0_l x1_l x2_l x3_l x4_l x5_l x6_l x7_l
+  let high := U64.mk x0_h x1_h x2_h x3_h x4_h x5_h x6_h x7_h
+
+  return ⟨ low, high ⟩
+
+def assumptions (x : U64 (F p)) := x.is_normalized
+
+def spec (offset : Fin 8) (input : U64 (F p)) (out: Outputs (F p)) :=
+  let ⟨x0, x1, x2, x3, x4, x5, x6, x7⟩ := input
+  let ⟨⟨x0_l, x1_l, x2_l, x3_l, x4_l, x5_l, x6_l, x7_l⟩,
+        ⟨x0_h, x1_h, x2_h, x3_h, x4_h, x5_h, x6_h, x7_h⟩⟩ := out
+  x0.val = x0_l.val + x0_h.val * 2^(offset.val) ∧
+  x1.val = x1_l.val + x1_h.val * 2^(offset.val) ∧
+  x2.val = x2_l.val + x2_h.val * 2^(offset.val) ∧
+  x3.val = x3_l.val + x3_h.val * 2^(offset.val) ∧
+  x4.val = x4_l.val + x4_h.val * 2^(offset.val) ∧
+  x5.val = x5_l.val + x5_h.val * 2^(offset.val) ∧
+  x6.val = x6_l.val + x6_h.val * 2^(offset.val) ∧
+  x7.val = x7_l.val + x7_h.val * 2^(offset.val)
+
+-- #eval! (u64_byte_decomposition (p:=p_babybear) 0) default |>.operations.local_length
+-- #eval! (u64_byte_decomposition (p:=p_babybear) 0) default |>.output
+def elaborated (offset : Fin 8) : ElaboratedCircuit (F p) U64 (Var Outputs (F p)) where
+  main := u64_byte_decomposition offset
+  local_length _ := 16
+  output _ i0 := {
+    low := ⟨var ⟨i0 + 0⟩, var ⟨i0 + 2⟩, var ⟨i0 + 4⟩, var ⟨i0 + 6⟩, var ⟨i0 + 8⟩, var ⟨i0 + 10⟩, var ⟨i0 + 12⟩, var ⟨i0 + 14⟩⟩,
+    high := ⟨var ⟨i0 + 1⟩, var ⟨i0 + 3⟩, var ⟨i0 + 5⟩, var ⟨i0 + 7⟩, var ⟨i0 + 9⟩, var ⟨i0 + 11⟩, var ⟨i0 + 13⟩, var ⟨i0 + 15⟩⟩
+  }
+
+theorem soundness (offset : Fin 8) : Soundness (F p) (circuit := elaborated offset) assumptions (spec offset) := by
+  intro i0 env x_var ⟨x0, x1, x2, x3, x4, x5, x6, x7⟩ h_input x_byte h_holds
+  simp [circuit_norm, elaborated, u64_byte_decomposition, ByteLookup, ByteTable.equiv, h_input] at h_holds
+  simp [subcircuit_norm, ByteDecomposition.circuit, ByteDecomposition.elaborated,
+    ByteDecomposition.assumptions, ByteDecomposition.spec, eval, circuit_norm] at h_holds
+
+  simp [assumptions, U64.is_normalized] at x_byte
+  simp [eval, circuit_norm] at h_input
+
+  simp only [spec, ↓ProvableStruct.eval_eq_eval_struct, ProvableStruct.eval, from_components,
+    ProvableStruct.eval.go, eval, from_elements, size, to_vars, to_elements, elaborated, add_zero,
+    ElaboratedCircuit.output, Vector.map_mk, List.map_toArray, List.map_cons, Expression.eval,
+    List.map_nil]
+  obtain ⟨h0, h1, h2, h3, h4, h5, h6, h7⟩ := h_input
+  simp [h0, h1, h2, h3, h4, h5, h6, h7, and_assoc] at h_holds
+  clear h0 h1 h2 h3 h4 h5 h6 h7
+
+  obtain ⟨ h0, h1, h2, h3, h4, h5, h6, h7 ⟩ := h_holds
+  simp_all only [Nat.reducePow, Nat.reduceAdd, gt_iff_lt, forall_const]
+  trivial
+
+
+theorem completeness (offset : Fin 8) : Completeness (F p) (circuit := elaborated offset) Outputs assumptions := by
+  rintro i0 env ⟨x0_var, x1_var, x2_var, x3_var, x4_var, x5_var, x6_var, x7_var⟩ henv ⟨x0, x1, x2, x3, x4, x5, x6, x7⟩ h_eval as
+  simp only [assumptions] at as
+  sorry
+
+def circuit (offset : Fin 8) : FormalCircuit (F p) U64 Outputs := {
+  elaborated offset with
+  main := u64_byte_decomposition offset
+  assumptions
+  spec := spec offset
+  soundness := soundness offset
+  completeness := completeness offset
+}
+end Gadgets.U64ByteDecomposition
